Inductive principles for terms and formulae.

theory/Util.v
@@ -1,4 +1,6 @@
 Set Warnings "-notation,-overridden,-parsing".
+Require Import Coq.Strings.String.
+Open Scope string_scope.
 Open Scope list_scope.
 
 Notation "x :: y" := (cons x y)
@@ -13,4 +15,37 @@ Fixpoint map {X Y : Type} (f: X->Y) (l: list X) : (list Y) :=
   | [] => []
   | h :: t => (f h) :: (map f t)
   end.
+
+Definition beq_string (s1 : string) (s2 : string) :=
+  if string_dec s1 s2 then true else false.
+
+Lemma beq_string_refl : forall (s : string),
+    beq_string s s = true.
+Proof.
+  intros. induction s as [| a s].
+  - reflexivity.
+  - unfold beq_string. destruct (string_dec (String a s) (String a s)).
+    + reflexivity.
+    + destruct n. reflexivity.
+Qed.
+
+Fixpoint beq_string_list (ss : list string) (ss': list string) :=
+  match ss with
+  | [] => match ss' with
+         | [] => true
+         | _ => false
+         end
+  | x :: xs => match ss' with
+              | y :: ys => andb (beq_string x y) (beq_string_list xs ys)
+              | _ => false
+              end
+  end.
+
+Theorem beq_string_list_refl : forall (ss : list string),
+    beq_string_list ss ss = true.
+Proof.
+  intros. induction ss.
+  - reflexivity.
+  - simpl. rewrite beq_string_refl. assumption.
+Qed.
 
