theory/Fol.v
@@ -2,20 +2,90 @@ Set Warnings "-notation-overridden,-parsing".
 Require Import Arith.
 Require Import Ascii.
 Require Import Strings.String.
+Require Import Coq.Lists.List.
+Import ListNotations.
 Require Import VHal.theory.Util.
-Open Scope string_scope. (* learn to use strings properly *)
+(* Open Scope string_scope. (* learn to use strings properly *) *)
 
-Inductive term : Type :=
+Inductive term : Set :=
 | Var : string -> term                           (* a name *)
-| Param : string * list string -> term           (* list of forbidden names *)
+| Param : string -> list string -> term           (* list of forbidden names *)
 | Bound : nat -> term                              (* an index *)
-| Fun : string * list term -> term.              (* name and argument list *)
+| Fun : string -> list term -> term.              (* name and argument list *)
 
-Inductive formula  : Type :=                   
-| Pred : string * list term -> formula           (* predicate name; arg list *)
-| Conn : string * list formula -> formula        (* connective; list of formulae *)
-| Quant : string * string * formula -> formula.  (* quantifier; var name; body *)
+Inductive formula : Set :=                   
+| Pred : string -> list term -> formula           (* predicate name; arg list *)
+| Conn : string -> list formula -> formula        (* connective; list of formulae *)
+| Quant : string -> string -> formula -> formula.  (* quantifier; var name; body *)
 
-Inductive goal : Type :=
+Inductive goal : Set :=
 | G : list formula * list formula -> goal.
 
+Section term_ind'.
+  Variable P : term -> Prop.
+
+  Hypothesis Var_case : forall s : string, P (Var s).
+  Hypothesis Param_case : forall (s : string) (ls : list string), P (Param s ls).
+  Hypothesis Bound_case : forall (n : nat), P (Bound n).
+  Hypothesis Fun_case : forall (s : string) (ls : list term),
+      Forall P ls -> P (Fun s ls).
+
+  Fixpoint term_ind' (t : term) : P t :=
+    match t with
+    | Var s => Var_case s
+    | Param s ls => Param_case s ls
+    | Bound n => Bound_case n
+    | Fun s ls => Fun_case s ls
+      ((fix list_term_ind (ls : list term) : Forall P ls :=
+          match ls with
+          | [] => Forall_nil _
+          | t :: ts => Forall_cons _ (term_ind' t) (list_term_ind ts)
+          end) ls)
+    end.
+End term_ind'.
+
+Section formula_ind'.
+  Variable P : formula -> Prop.
+
+  Hypothesis Pred_case : forall (s : string) (ls : list term), P (Pred s ls).
+  Hypothesis Conn_case : forall (s : string) (ls : list formula),
+      Forall P ls -> P (Conn s ls).
+  Hypothesis Quant_case : forall (s s' : string) (f : formula),
+      P f -> P (Quant s s' f).
+
+  Fixpoint formula_ind' (f : formula) : P f :=
+    match f with
+    | Pred s ls => Pred_case s ls
+    | Conn s ls => Conn_case s ls
+      ((fix list_formula_ind (ls : list formula) : Forall P ls :=
+          match ls with
+          | [] => Forall_nil _
+          | f :: fs => Forall_cons _ (formula_ind' f) (list_formula_ind fs)
+          end) ls)
+    | Quant s s' f => Quant_case s s' f (formula_ind' f)
+    end.
+End formula_ind'.
+
+(* https://bit.ly/2D7M02y *)
+Parameter term_eq_dec : forall (σ τ : term), { σ = τ } + { σ <> τ }.
+
+Definition beq_term (s : term) (t : term) :=
+  if term_eq_dec s t then true else false.
+
+(* https://bit.ly/2RNCENB *)
+Definition replace_one (u1 : term) (u2 : term) (t : term) :=
+  if beq_term t u1 then u2 else
+    let fix replace_one_aux (u1 : term) (u2 : term) (t : term) { struct t } : term :=
+        match t with
+        | Fun a args =>
+          (Fun a
+               ((fix replace_one_many_aux u1 u2 ts :=
+                   match ts with
+                   | [] => []
+                   | t :: ts =>
+                     (replace_one_aux u1 u2 t)
+                       :: (replace_one_many_aux u1 u2 ts)
+                   end) u1 u2 args))
+        | _ => t
+        end
+    in replace_one_aux u1 u2 t.
